

$$\begin{aligned}
 1.) \quad m(a + bx) &= \frac{1}{N} \sum_{i=1}^N (a + bx_i) \\
 &= \frac{1}{N} \left(\sum_{i=1}^N a + \sum_{i=1}^N bx_i \right) \\
 &= \frac{1}{N} (Na + b \sum_{i=1}^N x_i) \\
 &= a + b \left(\frac{1}{N} \sum_{i=1}^N x_i \right) \\
 &= a + b m(x)
 \end{aligned}$$

$$6.) \quad x = \{1, 2, 3\}$$

$$m(x) = \frac{1 + 2 + 3}{3} = 2$$

$$y = x^2$$

$$x^2 = \{1, 4, 9\}$$

$$m(x^2) = \frac{1 + 4 + 9}{3} = \frac{14}{3}$$

$$m(x)^2 = 2^2 = 4$$

$$\star m(x^2) \neq m(x)^2$$

$$\begin{aligned}
 2.) \quad \text{cov}(x, x) &= \frac{1}{N} \sum_{i=1}^N (x_i - m(x))(x_i - m(x)) \\
 &= \frac{1}{N} \sum_{i=1}^N (x_i - m(x))^2 = s^2
 \end{aligned}$$

\star by the def of sample variance

$$y = \sqrt{x}$$

$$\sqrt{x} = \{1, \sqrt{2}, \sqrt{3}\}$$

$$m(\sqrt{x}) = \frac{1 + \sqrt{2} + \sqrt{3}}{3} = 1.382$$

$$\sqrt{m(x)} = \sqrt{2} = 1.414$$

$$\star m(\sqrt{x}) \neq \sqrt{m(x)}$$

$$3.) \quad z = a + bY \quad \text{where} \quad z_i = a + by_i$$

$$m(z) = m(a + bY) = a + b m(Y)$$

$$\begin{aligned}
 \text{cov}(x, z) &= \frac{1}{N} \sum_{i=1}^N (x_i - m(x))(z_i - m(z)) \\
 &= \frac{1}{N} \sum_{i=1}^N (x_i - m(x)) [(a + by_i) - (a + b m(Y))] \\
 &= \frac{1}{N} \sum_{i=1}^N (x_i - m(x)) b(y_i - m(Y)) \\
 &= b \cdot \frac{1}{N} \sum_{i=1}^N (x_i - m(x))(y_i - m(Y)) \\
 &= b \text{cov}(x, Y)
 \end{aligned}$$

$$4.) \quad \star U = a + bX \quad V = a + bY$$

$$m(U) = a + b m(X) \quad m(V) = a + b m(Y)$$

$$u_i - m(U) = (a + bx_i) - (a + b m(x)) = b(x_i - m(x))$$

$$v_i - m(V) = (a + by_i) - (a + b m(Y)) = b(y_i - m(Y))$$

$$\begin{aligned}
 \text{cov}(U, V) &= \frac{1}{N} \sum_{i=1}^N (u_i - m(U))(v_i - m(V)) \\
 &= \frac{1}{N} \sum_{i=1}^N [b(x_i - m(x))] [b(y_i - m(Y))] \\
 &= b^2 \frac{1}{N} \sum_{i=1}^N (x_i - m(x))(y_i - m(Y)) \\
 &= b^2 \text{cov}(x, Y)
 \end{aligned}$$

$$5.) \quad \text{median}(a + bx) = a + b \text{med}(x)$$

\hookrightarrow yes this is true

$$IQR(x) = Q_3(x) - Q_1(x)$$

$$Q_1(a + bx) = a + b Q_1(x)$$

$$Q_3(a + bx) = a + b Q_3(x)$$

$$IQR(a + bx) = (a + b Q_3(x)) - (a + b Q_1(x))$$

$$= b(Q_3(x) - Q_1(x))$$

$$= b(IQR(x))$$

\hookrightarrow no, not true for IQR